examples/dynamic_isolation/External.v
@@ -43,15 +43,17 @@ End OriginalExternal.
 
 Module External <: External_sig.
   Import Common.
-  Inductive memory := imem | dmem | mainmem.
+
+  Inductive cache := imem | dmem.
 
   Inductive ext_fn_t' :=
-  | ext_mem (m: memory)
+  | ext_cache (c: cache)
+  | ext_mainmem
   | ext_uart_read
   | ext_uart_write
   | ext_led
+  | ext_ppp_bookkeeping
   .
-
 
   Definition ext_fn_t := ext_fn_t'.
   Definition led_input := maybe (bits_t 1).
@@ -101,25 +103,45 @@ Module External <: External_sig.
                         ("put_ready", bits_t 1);
                         ("get_response", struct_t ext_cache_mem_resp)] |}.
 
+  Definition Bookkeeping_row :=
+    {| struct_name := "Bookkeeping_row";
+       struct_fields := [("state", enum_t MSI);
+                         ("tag", cache_tag_t)]
+    |}.
+
+  Definition cache_type :=
+    {| enum_name := "cache_type";
+       enum_members := vect_of_list ["imem"; "dmem"];
+       enum_bitpatterns := vect_of_list [Ob~0; Ob~1] |}.
+
+  Definition bookkeeping_input :=
+    {| struct_name := "bookkeeping_input";
+       struct_fields := [("idx", bits_t log_num_sets);
+                         ("book", maybe (struct_t Bookkeeping_row));
+                         ("core_id", bits_t 1);
+                         ("cache_type", enum_t cache_type)
+                        ]
+    |}.
 
   Definition Sigma (fn: ext_fn_t) :=
     match fn with
-    | ext_mem imem => {$ struct_t cache_mem_input ~> struct_t cache_mem_output $}
-    | ext_mem dmem => {$ struct_t cache_mem_input ~> struct_t cache_mem_output $}
-    | ext_mem mainmem => {$ struct_t mem_input ~> struct_t mem_output $}
+    | ext_cache _ => {$ struct_t cache_mem_input ~> struct_t cache_mem_output $}
+    | ext_mainmem => {$ struct_t mem_input ~> struct_t mem_output $}
     | ext_uart_read => {$ bits_t 1 ~> uart_output $}
     | ext_uart_write => {$ uart_input ~> bits_t 1 $}
     | ext_led => {$ led_input ~> bits_t 1 $}
+    | ext_ppp_bookkeeping => {$ struct_t bookkeeping_input ~> maybe (struct_t Bookkeeping_row) $}
     end.
 
   Definition ext_fn_specs (fn: ext_fn_t) :=
     match fn with
-    | ext_mem imem => {| ef_name := "ext_mem_imem"; ef_internal := false |}
-    | ext_mem dmem => {| ef_name := "ext_mem_dmem"; ef_internal := false |}
-    | ext_mem main_mem => {| ef_name := "ext_mem_mainmem"; ef_internal := false |}
+    | ext_cache imem => {| ef_name := "ext_cache_imem"; ef_internal := false |}
+    | ext_cache dmem => {| ef_name := "ext_cache_dmem"; ef_internal := false |}
+    | ext_mainmem => {| ef_name := "ext_mainmem"; ef_internal := false |}
     | ext_uart_write => {| ef_name := "ext_uart_write"; ef_internal := false |}
     | ext_uart_read => {| ef_name := "ext_uart_read"; ef_internal := false |}
     | ext_led => {| ef_name := "ext_led"; ef_internal := false |}
+    | ext_ppp_bookkeeping => {| ef_name := "ext_ppp_bookkeeping"; ef_internal := false |}
     end.
 
   Instance Show_ext_fn_t : Show ext_fn_t := _.
